examples/xlrup_checker/array/xlrup_arrayFullProgScript.sml
@@ -1,0 +1,708 @@
+(*
+  This builds the cake_xlrup proof checker
+*)
+open preamble basis UnsafeProofTheory xlrupTheory xlrup_listTheory xlrup_parsingTheory xlrup_arrayProgTheory cnf_xorTheory;
+
+val _ = new_theory "xlrup_arrayFullProg"
+
+val _ = temp_delsimps ["NORMEQ_CONV"]
+val _ = diminish_srw_ss ["ABBREV"]
+val _ = set_trace "BasicProvers.var_eq_old" 1
+
+val _ = translation_extends"xlrup_arrayProg";
+
+val xlet_autop = xlet_auto >- (TRY( xcon) >> xsimpl)
+
+val _ = translate parse_header_line_def;
+
+val parse_header_line_side = Q.prove(`
+   ∀x. parse_header_line_side x= T`,
+  rw[definition"parse_header_line_side_def"]>>
+  intLib.ARITH_TAC)
+  |> update_precondition;
+
+val _ = translate parse_lits_aux_def;
+val _ = translate parse_clause_def;
+val _ = translate parse_xor_def;
+val _ = translate parse_line_def;
+
+val _ = translate nocomment_line_def;
+
+val format_dimacs_failure_def = Define`
+  format_dimacs_failure (lno:num) s =
+  strlit "c DIMACS parse failed at line: " ^ toString lno ^ strlit ". Reason: " ^ s ^ strlit"\n"`
+
+val _ = translate format_dimacs_failure_def;
+
+val b_inputLineTokens_specialize =
+  b_inputLineTokens_spec_lines
+  |> Q.GEN `f` |> Q.SPEC`blanks`
+  |> Q.GEN `fv` |> Q.SPEC`blanks_v`
+  |> Q.GEN `g` |> Q.ISPEC`tokenize`
+  |> Q.GEN `gv` |> Q.ISPEC`tokenize_v`
+  |> Q.GEN `a` |> Q.ISPEC`SUM_TYPE STRING_TYPE INT`
+  |> SIMP_RULE std_ss [blanks_v_thm,tokenize_v_thm,blanks_def] ;
+
+val parse_body_arr = process_topdecs`
+  fun parse_body_arr lno maxvar fd cacc xacc =
+  case TextIO.b_inputLineTokens fd blanks tokenize of
+    None => Inr (List.rev cacc, List.rev xacc)
+  | Some l =>
+    if nocomment_line l then
+      (case parse_line maxvar l of
+        None => Inl (format_failure lno "failed to parse line")
+      | Some (Inl cl) =>
+        parse_body_arr (lno+1) maxvar fd (cl::cacc) xacc
+      | Some (Inr xl) =>
+        parse_body_arr (lno+1) maxvar fd cacc (xl::xacc)
+      )
+    else parse_body_arr (lno+1) maxvar fd cacc xacc` |> append_prog;
+
+Overload "LL_LIT_TYPE" = ``LIST_TYPE (LIST_TYPE (CNF_XOR_LIT_TYPE NUM))``
+
+Theorem parse_body_arr_spec:
+  !lines fd fdv fs maxvar maxvarv cacc caccv xacc xaccv lno lnov.
+  NUM lno lnov ∧
+  NUM maxvar maxvarv ∧
+  LL_LIT_TYPE cacc caccv ∧
+  LL_LIT_TYPE xacc xaccv
+  ⇒
+  app (p : 'ffi ffi_proj)
+    ^(fetch_v "parse_body_arr" (get_ml_prog_state()))
+    [lnov; maxvarv; fdv; caccv; xaccv]
+    (STDIO fs * INSTREAM_LINES fd fdv lines fs)
+    (POSTv v.
+      &
+      (∃err. SUM_TYPE STRING_TYPE
+        (PAIR_TYPE LL_LIT_TYPE LL_LIT_TYPE)
+      (case parse_body maxvar
+        (FILTER nocomment_line (MAP toks lines)) cacc xacc of
+        NONE => INL err
+      | SOME x => INR x) v) *
+      SEP_EXISTS k lines'.
+         STDIO (forwardFD fs fd k) * INSTREAM_LINES fd fdv lines' (forwardFD fs fd k))
+Proof
+  Induct
+  \\ simp []
+  \\ xcf "parse_body_arr" (get_ml_prog_state ())
+  THEN1 (
+    xlet ‘(POSTv v.
+            SEP_EXISTS k.
+                STDIO (forwardFD fs fd k) *
+                INSTREAM_LINES fd fdv [] (forwardFD fs fd k) *
+                &OPTION_TYPE (LIST_TYPE (SUM_TYPE STRING_TYPE INT)) NONE v)’
+    THEN1 (
+      xapp_spec b_inputLineTokens_specialize
+      \\ qexists_tac `emp`
+      \\ qexists_tac ‘[]’
+      \\ qexists_tac ‘fs’
+      \\ qexists_tac ‘fd’ \\ xsimpl \\ fs [])
+    \\ gvs[OPTION_TYPE_def]
+    \\ xmatch
+    \\ simp[parse_body_def]
+    \\ rpt xlet_autop
+    \\ xcon \\ xsimpl
+    \\ simp[SUM_TYPE_def,PAIR_TYPE_def]
+    \\ qexists_tac ‘k’ \\ xsimpl
+    \\ qexists_tac `[]` \\ xsimpl)
+  \\ xlet ‘(POSTv v.
+            SEP_EXISTS k.
+                STDIO (forwardFD fs fd k) *
+                INSTREAM_LINES fd fdv lines (forwardFD fs fd k) *
+                & OPTION_TYPE (LIST_TYPE (SUM_TYPE STRING_TYPE INT)) (SOME (toks h)) v)’
+    THEN1 (
+      xapp_spec b_inputLineTokens_specialize
+      \\ qexists_tac `emp`
+      \\ qexists_tac ‘h::lines’
+      \\ qexists_tac ‘fs’
+      \\ qexists_tac ‘fd’ \\ xsimpl \\ fs []
+      \\ rw [] \\ qexists_tac ‘x’ \\ xsimpl
+      \\ simp[toks_def])
+  \\ gvs[OPTION_TYPE_def]
+  \\ xmatch \\ fs []
+  \\ xlet_autop
+  \\ reverse IF_CASES_TAC
+  >- (
+    xif >> asm_exists_tac>>xsimpl>>
+    xlet_autop>>
+    xapp>> xsimpl>>
+    rpt(first_x_assum (irule_at Any))>>
+    qexists_tac`forwardFD fs fd k`>>
+    qexists_tac`fd`>>xsimpl>>
+    rw[]>>
+    qexists_tac`k+x`>>
+    simp[GSYM fsFFIPropsTheory.forwardFD_o]>>
+    qexists_tac`x'`>>xsimpl>>
+    metis_tac[])>>
+  xif>> asm_exists_tac>>simp[]>>
+  xlet_autop>>
+  simp[parse_body_def]>>
+  Cases_on`parse_line maxvar (toks h)`>>fs[OPTION_TYPE_def]
+  >- (
+    xmatch>>
+    xlet_autop>>
+    xcon>>
+    xsimpl>>
+    qexists_tac`k`>> qexists_tac`lines`>>xsimpl>>
+    simp[SUM_TYPE_def]>>
+    metis_tac[])>>
+  Cases_on`x`>>fs[SUM_TYPE_def]>>
+  rename1`LIST_TYPE _ ll _`>>
+  xmatch>>
+  xlet_autop>>
+  xlet_autop>>
+  xapp>>
+  xsimpl>>
+  rpt(first_x_assum (irule_at Any))
+  >- (
+    qexists_tac`forwardFD fs fd k`>>
+    qexists_tac`fd`>>
+    qexists_tac`ll::cacc`>>
+    xsimpl>>
+    simp[LIST_TYPE_def,forwardFD_o]>>rw[]>>
+    qexists_tac`k+x`>>
+    qexists_tac`x'`>>
+    xsimpl>>
+    metis_tac[])
+  >- (
+    qexists_tac`ll::xacc`>>
+    qexists_tac`forwardFD fs fd k`>>
+    qexists_tac`fd`>>
+    xsimpl>>
+    simp[LIST_TYPE_def,forwardFD_o]>>rw[]>>
+    qexists_tac`k+x`>>
+    qexists_tac`x'`>>
+    xsimpl>>
+    metis_tac[])
+QED
+
+val parse_cnf_xor_toks_arr = process_topdecs`
+  fun parse_cnf_xor_toks_arr lno fd =
+  case TextIO.b_inputLineTokens fd blanks tokenize of
+    None => Inl (format_failure lno "failed to find header")
+  | Some l =>
+    if nocomment_line l then
+      (case parse_header_line l of
+        None => Inl (format_failure lno "failed to parse header")
+      | Some res => case res of (vars,ncx) =>
+        (case parse_body_arr lno vars fd [] [] of
+          Inl fail => Inl fail
+        | Inr (cacc,xacc) =>
+          if List.length cacc + List.length xacc = ncx then
+            Inr (vars,(ncx,(cacc,xacc)))
+          else
+            Inl (format_failure lno "incorrect number of clauses / xors")))
+    else parse_cnf_xor_toks_arr (lno+1) fd` |> append_prog;
+
+Theorem parse_cnf_xor_toks_arr_spec:
+  !lines fd fdv fs lno lnov.
+  NUM lno lnov
+  ⇒
+  app (p : 'ffi ffi_proj)
+    ^(fetch_v "parse_cnf_xor_toks_arr" (get_ml_prog_state()))
+    [lnov; fdv]
+    (STDIO fs * INSTREAM_LINES fd fdv lines fs)
+    (POSTv v.
+      & (∃err. SUM_TYPE STRING_TYPE
+        (PAIR_TYPE NUM (PAIR_TYPE NUM
+          (PAIR_TYPE LL_LIT_TYPE LL_LIT_TYPE)))
+      (case parse_cnf_xor_toks (MAP toks lines) of
+        NONE => INL err
+      | SOME x => INR x) v) *
+      SEP_EXISTS k lines'.
+         STDIO (forwardFD fs fd k) * INSTREAM_LINES fd fdv lines' (forwardFD fs fd k))
+Proof
+  Induct
+  \\ simp []
+  \\ xcf "parse_cnf_xor_toks_arr" (get_ml_prog_state ())
+  THEN1 (
+    xlet ‘(POSTv v.
+            SEP_EXISTS k.
+                STDIO (forwardFD fs fd k) *
+                INSTREAM_LINES fd fdv [] (forwardFD fs fd k) *
+                &OPTION_TYPE (LIST_TYPE (SUM_TYPE STRING_TYPE INT)) NONE v)’
+    THEN1 (
+      xapp_spec b_inputLineTokens_specialize
+      \\ qexists_tac `emp`
+      \\ qexists_tac ‘[]’
+      \\ qexists_tac ‘fs’
+      \\ qexists_tac ‘fd’ \\ xsimpl \\ fs [])
+    \\ fs [std_preludeTheory.OPTION_TYPE_def] \\ rveq \\ fs []
+    \\ xmatch \\ fs []
+    \\ simp[parse_cnf_xor_toks_def]
+    \\ xlet_autop
+    \\ xcon \\ xsimpl
+    \\ simp[SUM_TYPE_def]
+    \\ qexists_tac ‘k’ \\ xsimpl
+    \\ qexists_tac `[]` \\ xsimpl
+    \\ metis_tac[])
+  \\ xlet ‘(POSTv v.
+            SEP_EXISTS k.
+                STDIO (forwardFD fs fd k) *
+                INSTREAM_LINES fd fdv lines (forwardFD fs fd k) *
+                & OPTION_TYPE (LIST_TYPE (SUM_TYPE STRING_TYPE INT)) (SOME (toks h)) v)’
+    THEN1 (
+      xapp_spec b_inputLineTokens_specialize
+      \\ qexists_tac `emp`
+      \\ qexists_tac ‘h::lines’
+      \\ qexists_tac ‘fs’
+      \\ qexists_tac ‘fd’ \\ xsimpl \\ fs []
+      \\ rw [] \\ qexists_tac ‘x’ \\ xsimpl
+      \\ simp[toks_def])
+  \\ fs [std_preludeTheory.OPTION_TYPE_def] \\ rveq \\ fs []
+  \\ xmatch \\ fs []
+  \\ xlet_autop
+  \\ simp[parse_cnf_xor_toks_def]
+  \\ reverse IF_CASES_TAC
+  >- (
+    xif >> asm_exists_tac>>xsimpl>>
+    xlet_autop>>
+    xapp>> xsimpl>>
+    asm_exists_tac>> simp[]>>
+    qexists_tac`emp`>>xsimpl>>
+    qexists_tac`forwardFD fs fd k`>>
+    qexists_tac`fd`>>xsimpl>>
+    rw[]>>
+    fs[parse_cnf_xor_toks_def]>>
+    qexists_tac`k+x`>>
+    simp[GSYM fsFFIPropsTheory.forwardFD_o]>>
+    qexists_tac`x'`>>xsimpl>>
+    metis_tac[])>>
+  xif>> asm_exists_tac>>simp[]>>
+  xlet_autop>>
+  Cases_on`parse_header_line (toks h)`>>fs[OPTION_TYPE_def]
+  >- (
+    xmatch>>
+    xlet_autop>>
+    xcon>>
+    xsimpl>>
+    qexists_tac`k`>> qexists_tac`lines`>>xsimpl>>
+    simp[SUM_TYPE_def]>>
+    metis_tac[])>>
+  xmatch>>
+  Cases_on`x`>>fs[PAIR_TYPE_def]>>
+  xmatch>>
+  rpt xlet_autop>>
+  xlet `(POSTv v.
+      & (∃err. SUM_TYPE STRING_TYPE
+        (PAIR_TYPE LL_LIT_TYPE LL_LIT_TYPE)
+      (case parse_body q (FILTER nocomment_line (MAP toks lines)) [] [] of
+        NONE => INL err
+      | SOME x => INR x) v) *
+      SEP_EXISTS k lines'.
+         STDIO (forwardFD fs fd k) * INSTREAM_LINES fd fdv lines' (forwardFD fs fd k))`
+  >- (
+    xapp>>xsimpl>>
+    qexists_tac`emp`>>
+    rpt(first_x_assum (irule_at Any))>>
+    qexists_tac`[]`>>
+    qexists_tac`lines`>>
+    qexists_tac`forwardFD fs fd k`>>
+    qexists_tac`fd`>>xsimpl>>
+    qexists_tac`[]`>>simp[LIST_TYPE_def]>>
+    rw[]>>
+    qexists_tac`k+x`>>
+    simp[GSYM fsFFIPropsTheory.forwardFD_o]>>
+    qexists_tac`x'`>>xsimpl>>
+    metis_tac[])>>
+  pop_assum mp_tac>> TOP_CASE_TAC>>fs[OPTION_TYPE_def]
+  >- (
+    rw[]>>fs[SUM_TYPE_def]>>
+    xmatch>>
+    xcon>>
+    xsimpl>>
+    qexists_tac`k`>>qexists_tac`lines'`>>xsimpl>>
+    metis_tac[])>>
+  strip_tac>>fs[SUM_TYPE_def]>>
+  Cases_on`x`>>fs[PAIR_TYPE_def]>>
+  xmatch>>
+  rpt xlet_autop>>
+  rw[]>> xif
+  >- (
+    asm_exists_tac>>simp[]>>
+    rpt xlet_autop>>
+    xcon>>xsimpl>>
+    simp[SUM_TYPE_def,PAIR_TYPE_def]>>
+    qexists_tac`k`>>qexists_tac`lines'`>>xsimpl)>>
+  asm_exists_tac>>simp[]>>
+  xlet_autop>>
+  xcon>>
+  xsimpl>>
+  qexists_tac`k`>>
+  qexists_tac`lines'`>>
+  simp[SUM_TYPE_def,PAIR_TYPE_def]>>
+  xsimpl>>
+  metis_tac[]
+QED
+
+(* parse_cnf_xor_toks with simple wrapper *)
+val parse_full = (append_prog o process_topdecs) `
+  fun parse_full fname =
+  let
+    val fd = TextIO.b_openIn fname
+    val res = parse_cnf_xor_toks_arr 0 fd
+    val close = TextIO.b_closeIn fd;
+  in
+    res
+  end
+  handle TextIO.BadFileName => Inl (notfound_string fname)`;
+
+Theorem parse_full_spec:
+  STRING_TYPE f fv ∧
+  validArg f ∧
+  hasFreeFD fs
+  ⇒
+  app (p:'ffi ffi_proj) ^(fetch_v"parse_full"(get_ml_prog_state()))
+    [fv]
+    (STDIO fs)
+    (POSTv v.
+    & (∃err. (SUM_TYPE STRING_TYPE (PAIR_TYPE NUM (PAIR_TYPE NUM
+        (PAIR_TYPE LL_LIT_TYPE LL_LIT_TYPE)))
+    (if inFS_fname fs f then
+    (case parse_cnf_xor_toks (MAP toks (all_lines fs f)) of
+      NONE => INL err
+    | SOME x => INR x)
+    else INL err) v)) * STDIO fs)
+Proof
+  rw[]>>
+  xcf"parse_full"(get_ml_prog_state()) >>
+  fs[validArg_def]>>
+  reverse (Cases_on `STD_streams fs`)
+  >- (fs [TextIOProofTheory.STDIO_def] \\ xpull) >>
+  reverse (Cases_on`consistentFS fs`)
+  >- (fs [STDIO_def,IOFS_def,wfFS_def,consistentFS_def] \\ xpull \\ metis_tac[]) >>
+  reverse (Cases_on `inFS_fname fs f`) >> simp[]
+  >- (
+    xhandle`POSTe ev.
+      &BadFileName_exn ev *
+      &(~inFS_fname fs f) *
+      STDIO fs`
+    >-
+      (xlet_auto_spec (SOME b_openIn_STDIO_spec) \\ xsimpl)
+    >>
+      fs[BadFileName_exn_def]>>
+      xcases>>rw[]>>
+      xlet_auto>>xsimpl>>
+      xcon>>xsimpl>>
+      simp[SUM_TYPE_def]>>metis_tac[])>>
+  qmatch_goalsub_abbrev_tac`$POSTv Qval`>>
+  xhandle`$POSTv Qval` \\ xsimpl >>
+  qunabbrev_tac`Qval`>>
+  xlet_auto_spec (SOME b_openIn_spec_lines) \\ xsimpl >>
+  qmatch_goalsub_abbrev_tac`STDIO fss`>>
+  qmatch_goalsub_abbrev_tac`INSTREAM_LINES fdd fddv lines fss`>>
+  xlet`(POSTv v.
+      & (∃err. SUM_TYPE STRING_TYPE (PAIR_TYPE NUM (PAIR_TYPE NUM
+        (PAIR_TYPE LL_LIT_TYPE LL_LIT_TYPE)))
+      (case parse_cnf_xor_toks (MAP toks lines) of
+        NONE => INL err
+      | SOME x => INR x) v) *
+      SEP_EXISTS k lines'.
+         STDIO (forwardFD fss fdd k) * INSTREAM_LINES fdd fddv lines' (forwardFD fss fdd k))`
+  >- (
+    xapp>>xsimpl>>
+    qexists_tac`emp`>>qexists_tac`lines`>>
+    qexists_tac`fss`>>qexists_tac`fdd`>>xsimpl>>
+    rw[]>>
+    qexists_tac`x`>>qexists_tac`x'`>>xsimpl>>
+    metis_tac[])>>
+  xlet `POSTv v. STDIO fs`
+  >- (
+    xapp_spec b_closeIn_spec_lines >>
+    qexists_tac `emp`>>
+    qexists_tac `lines'` >>
+    qexists_tac `forwardFD fss fdd k` >>
+    qexists_tac `fdd` >>
+    conj_tac THEN1
+     (unabbrev_all_tac
+      \\ imp_res_tac fsFFIPropsTheory.nextFD_ltX \\ fs []
+      \\ imp_res_tac fsFFIPropsTheory.STD_streams_nextFD \\ fs []) >>
+    xsimpl>>
+    `validFileFD fdd (forwardFD fss fdd k).infds` by
+      (unabbrev_all_tac>> simp[validFileFD_forwardFD]
+       \\ imp_res_tac fsFFIPropsTheory.nextFD_ltX \\ fs []
+       \\ match_mp_tac validFileFD_nextFD \\ fs []) >>
+    xsimpl >> rw [] >>
+    imp_res_tac (DECIDE ``n<m:num ==> n <= m``) >>
+    imp_res_tac fsFFIPropsTheory.nextFD_leX \\ fs [] >>
+    drule fsFFIPropsTheory.openFileFS_ADELKEY_nextFD >>
+    fs [Abbr`fss`] \\ xsimpl)>>
+  xvar>>
+  xsimpl>>
+  metis_tac[]
+QED
+
+val usage_string = ‘
+
+Usage:  cake_xlrup <CNF XOR formula file> <XLRUP proof file>
+Run XLRUP unsatisfiability proof checking
+
+’
+
+fun drop_until p [] = []
+  | drop_until p (x::xs) = if p x then x::xs else drop_until p xs;
+
+val usage_string_tm =
+  usage_string |> hd |> (fn QUOTE s => s) |> explode
+  |> drop_until (fn c => c = #"\n") |> tl |> implode
+  |> stringSyntax.fromMLstring;
+
+Definition usage_string_def:
+  usage_string = strlit ^usage_string_tm
+End
+
+val r = translate usage_string_def;
+
+(* TODO: XORs *)
+val r = translate conv_lit_def;
+val r = translate conv_cfml_def;
+
+(*
+  Checker takes up to 2 arguments:
+  2 args (CNF XOR file, proof file):
+    parse CNF XOR, run proof, report UNSAT (or error)
+*)
+
+val check_unsat_2 = (append_prog o process_topdecs) `
+  fun check_unsat_2 f1 f2 =
+  case parse_full f1 of
+    Inl err => TextIO.output TextIO.stdErr err
+  | Inr (mv,(ncx,(cfml,xfml))) =>
+  let val cfml = conv_cfml cfml
+      val one = 1
+      val carr = Array.array (2*ncx) None
+      val carr = fill_arr carr one cfml
+      val xarr = Array.array 0 None
+      val bnd = 2*mv + 3
+  in
+    case check_unsat' carr xarr f2 bnd of
+      Inl err => TextIO.output TextIO.stdErr err
+    | Inr b =>
+      if b then
+        TextIO.print "s VERIFIED UNSAT\n"
+      else
+        TextIO.output TextIO.stdErr "c empty clause not derived at end of proof\n"
+  end`
+
+val check_unsat = (append_prog o process_topdecs) `
+  fun check_unsat u =
+  case CommandLine.arguments () of
+    [f1,f2] => check_unsat_2 f1 f2
+  | _ => TextIO.output TextIO.stdErr usage_string`
+
+(* We verify each argument type separately *)
+val b_inputAllTokensFrom_spec_specialize =
+  b_inputAllTokensFrom_spec
+  |> Q.GEN `f` |> Q.SPEC`blanks`
+  |> Q.GEN `fv` |> Q.SPEC`blanks_v`
+  |> Q.GEN `g` |> Q.ISPEC`tokenize`
+  |> Q.GEN `gv` |> Q.ISPEC`tokenize_v`
+  |> Q.GEN `a` |> Q.ISPEC`SUM_TYPE STRING_TYPE INT`
+  |> REWRITE_RULE [blanks_v_thm,tokenize_v_thm,blanks_def] ;
+
+val check_unsat_2_sem_def = Define`
+  check_unsat_2_sem fs f1 f2 err =
+  if inFS_fname fs f1 then
+  (case parse_cnf_xor_toks (MAP toks (all_lines fs f1)) of
+    NONE => add_stderr fs err
+  | SOME (mv,ncl,cfml,xfml) =>
+    let cfml = conv_cfml cfml in
+    if inFS_fname fs f2 then
+      case parse_xlrups (all_lines fs f2) of
+        SOME xlrups =>
+        let cfmlls = enumerate 1 cfml in
+        let base = REPLICATE (2*ncl) NONE in
+        let bnd = 2*mv+3 in
+        let cupd = FOLDL (λacc (i,v). resize_update_list acc NONE (SOME v) i) base cfmlls in
+          if check_xlrups_unsat_list xlrups cupd ([]:strxor option list)
+            (REPLICATE bnd w8z) then
+            add_stdout fs (strlit "s VERIFIED UNSAT\n")
+          else
+            add_stderr fs err
+      | NONE => add_stderr fs err
+    else add_stderr fs err)
+  else add_stderr fs err`
+
+val err_tac = xapp_spec output_stderr_spec \\ xsimpl>>
+    asm_exists_tac>>xsimpl>>
+    qexists_tac`emp`>>xsimpl>>
+    qexists_tac`fs`>>xsimpl>>
+    rw[]>>qexists_tac`err`>>xsimpl;
+
+Theorem check_unsat_2_spec:
+  STRING_TYPE f1 f1v ∧ validArg f1 ∧
+  STRING_TYPE f2 f2v ∧ validArg f2 ∧
+  hasFreeFD fs
+  ⇒
+  app (p:'ffi ffi_proj) ^(fetch_v"check_unsat_2"(get_ml_prog_state()))
+    [f1v; f2v]
+    (STDIO fs)
+    (POSTv uv. &UNIT_TYPE () uv *
+    SEP_EXISTS err. STDIO (check_unsat_2_sem fs f1 f2 err))
+Proof
+  rw[]>>
+  xcf "check_unsat_2" (get_ml_prog_state ())>>
+  xlet_autop>>
+  simp[check_unsat_2_sem_def]>>
+  reverse TOP_CASE_TAC>>fs[]
+  >- (
+    fs[SUM_TYPE_def]>>xmatch>>
+    err_tac)>>
+  TOP_CASE_TAC>> fs[SUM_TYPE_def]
+  >- (xmatch>> err_tac)>>
+  PairCases_on`x`>>fs[SUM_TYPE_def,PAIR_TYPE_def]>>
+  xmatch>>
+  rename1`_ = SOME (_,_,cfml,xfml)`>>
+  xlet_autop>>
+  xlet`POSTv v. &NUM 1 v * STDIO fs` >- (xlit>>xsimpl)>>
+  rw[]>>
+  (drule_at (Pos (hd o tl))) fill_arr_spec>>
+  (* help instantiate fill_arr_spec *)
+  `LIST_REL (OPTION_TYPE (LIST_TYPE INT)) (REPLICATE (2 * x1) NONE)
+        (REPLICATE (2 * x1) (Conv (SOME (TypeStamp "None" 2)) []))` by
+    simp[LIST_REL_REPLICATE_same,OPTION_TYPE_def]>>
+  disch_then drule>>
+  disch_then drule>>
+  rw[]>>
+  rpt xlet_autop>>
+  simp[check_xlrups_unsat_list_def]>>
+  qmatch_goalsub_abbrev_tac`check_xlrups_list _ a b c`>>
+  xlet`POSTv v.
+    STDIO fs *
+    SEP_EXISTS err.
+     &SUM_TYPE STRING_TYPE BOOL
+      (if inFS_fname fs f2 then
+         (case parse_xlrups (all_lines fs f2) of
+            NONE => INL err
+          | SOME xlrups =>
+            (case check_xlrups_list xlrups a b c of
+             NONE => INL err
+           | SOME (cfml', xfml') =>
+           INR (contains_emp_list cfml')))
+       else INL err) v`
+  >- (
+    xapp_spec (GEN_ALL check_unsat'_spec)>>
+    cheat)
+    (*xsimpl>>
+    asm_exists_tac>>simp[]>>
+    fs[FILENAME_def,validArg_def]>>
+    asm_exists_tac>>simp[]>>
+    asm_exists_tac>>simp[]>>
+    simp[Once (METIS_PROVE [] ``P ∧ Q ∧ C ⇔ Q ∧ C ∧ P``)]>>
+    asm_exists_tac>>simp[]>>
+    qexists_tac`emp`>>xsimpl>>
+    reverse CONJ_TAC>- (
+      cheat)>>
+    fs[LENGTH_enumerate,rev_enum_full_rev_enumerate,Abbr`b`]>>
+    rw[]>>
+    qexists_tac`x`>>simp[]
+    metis_tac[] *)>>
+  reverse TOP_CASE_TAC>>simp[]
+  >- (fs[SUM_TYPE_def]>>xmatch>>err_tac)>>
+  TOP_CASE_TAC>>fs[SUM_TYPE_def]
+  >- (xmatch>>err_tac)>>
+  Cases_on`check_xlrups_list x a b c`>>fs[SUM_TYPE_def]
+  >- (xmatch>>err_tac)>>
+  Cases_on`x'`>>fs[]>>
+  fs[SUM_TYPE_def]>>
+  xmatch>>
+  xif
+  >- (
+    xapp_spec print_spec >> xsimpl
+    \\ qexists_tac`emp`
+    \\ qexists_tac`fs`>>xsimpl)
+  >- (
+    gs[GSYM quantHeuristicsTheory.IS_SOME_EQ_NOT_NONE,IS_SOME_EXISTS,OPTION_TYPE_def]>>
+    xapp_spec output_stderr_spec \\ xsimpl>>
+    qexists_tac`emp`>>xsimpl>>
+    qexists_tac`fs`>>xsimpl>>
+    rw[]>>
+    qmatch_goalsub_abbrev_tac`_ _ err`>>
+    qexists_tac`err`>>xsimpl)
+QED
+
+val check_unsat_sem_def = Define`
+  check_unsat_sem cl fs err =
+  case TL cl of
+  | [f1;f2] => check_unsat_2_sem fs f1 f2 err
+  | _ => add_stderr fs err`
+
+Theorem check_unsat_spec:
+   hasFreeFD fs
+   ⇒
+   app (p:'ffi ffi_proj) ^(fetch_v"check_unsat"(get_ml_prog_state()))
+     [Conv NONE []]
+     (COMMANDLINE cl * STDIO fs)
+     (POSTv uv. &UNIT_TYPE () uv *
+     COMMANDLINE cl * SEP_EXISTS err. STDIO (check_unsat_sem cl fs err))
+Proof
+  xcf"check_unsat"(get_ml_prog_state())>>
+  reverse(Cases_on`wfcl cl`) >- (fs[COMMANDLINE_def] \\ xpull)>>
+  rpt xlet_autop >>
+  Cases_on `cl` >- fs[wfcl_def] >>
+  simp[check_unsat_sem_def]>>
+  every_case_tac>>fs[LIST_TYPE_def]>>xmatch>>
+  qmatch_asmsub_abbrev_tac`wfcl cl`
+  >- (
+    xapp_spec output_stderr_spec \\ xsimpl>>
+    qexists_tac`COMMANDLINE cl`>>xsimpl>>
+    qexists_tac `usage_string` >> simp [theorem "usage_string_v_thm"] >>
+    qexists_tac`fs`>>xsimpl>>
+    rw[]>>qexists_tac`usage_string`>>xsimpl)
+  >- (
+    xapp_spec output_stderr_spec \\ xsimpl>>
+    qexists_tac`COMMANDLINE cl`>>xsimpl>>
+    qexists_tac `usage_string` >> simp [theorem "usage_string_v_thm"] >>
+    qexists_tac`fs`>>xsimpl>>
+    rw[]>>qexists_tac`usage_string`>>xsimpl)
+  >- (
+    xapp>>xsimpl>>
+    qexists_tac`COMMANDLINE cl`>>xsimpl>>
+    fs[wfcl_def,Abbr`cl`]>>
+    qexists_tac`fs`>>
+    qexists_tac`h''`>>
+    qexists_tac`h'`>>
+    xsimpl>>rw[]>>
+    qexists_tac`x`>>xsimpl)
+  >- (
+    xapp_spec output_stderr_spec \\ xsimpl>>
+    qexists_tac`COMMANDLINE cl`>>xsimpl>>
+    qexists_tac `usage_string` >> simp [theorem "usage_string_v_thm"] >>
+    qexists_tac`fs`>>xsimpl>>
+    rw[]>>qexists_tac`usage_string`>>xsimpl)
+QED
+
+Theorem check_unsat_whole_prog_spec2:
+   hasFreeFD fs ⇒
+   whole_prog_spec2 check_unsat_v cl fs NONE (λfs'. ∃err. fs' = check_unsat_sem cl fs err)
+Proof
+  rw[basis_ffiTheory.whole_prog_spec2_def]
+  \\ match_mp_tac (MP_CANON (DISCH_ALL (MATCH_MP app_wgframe (UNDISCH check_unsat_spec))))
+  \\ xsimpl
+  \\ rw[PULL_EXISTS]
+  \\ qexists_tac`check_unsat_sem cl fs x`
+  \\ qexists_tac`x`
+  \\ xsimpl
+  \\ rw[check_unsat_sem_def,check_unsat_2_sem_def]
+  \\ every_case_tac
+  \\ simp[GSYM add_stdo_with_numchars,with_same_numchars]
+QED
+
+local
+
+val name = "check_unsat"
+val (sem_thm,prog_tm) =
+  whole_prog_thm (get_ml_prog_state()) name (UNDISCH check_unsat_whole_prog_spec2)
+val check_unsat_prog_def = Define`check_unsat_prog = ^prog_tm`;
+
+in
+
+Theorem check_unsat_semantics =
+  sem_thm
+  |> REWRITE_RULE[GSYM check_unsat_prog_def]
+  |> DISCH_ALL
+  |> SIMP_RULE(srw_ss())[GSYM CONJ_ASSOC,AND_IMP_INTRO];
+
+end
+
+val _ = export_theory();
